ironfleet/src/Dafny/Distributed/Impl/WS/HostState.i.dfy
@@ -1,0 +1,90 @@
+include "../../Protocol/WS/Host.i.dfy"
+include "ConstantsState.i.dfy"
+include "../../Common/Logic/Option.i.dfy"
+include "CMessage.i.dfy"
+include "PacketParsing.i.dfy"
+
+module SHT__HostState_i {
+import opened WS__Host_i
+import opened Logic__Option_i
+import opened WS__ConstantsState_i
+import opened WS__CMessage_i
+import opened WS__PacketParsing_i
+
+datatype HostState = HostState(
+    constants:ConstantsState,
+    fs:FileSystemState,
+    me:EndPoint,
+    ghost receivedRequests:seq<AppRequest>
+)
+
+predicate HostStateIsAbstractable(host:HostState)
+{
+       ConstantsStateIsAbstractable(host.constants)
+    && EndPointIsAbstractable(host.me)
+    && true // file system state goes straight across
+}
+
+function AbstractifyHostStateToHost(host:HostState) : Host
+    requires HostStateIsAbstractable(host)
+{
+    Host(AbstractifyToConstants(host.constants),
+        host.fs,
+        AbstractifyEndPointToNodeIdentity(host.me), 
+        host.receivedRequests)
+}
+
+
+predicate HostStateIsValid(host:HostState)
+{
+       HostStateIsAbstractable(host)
+    && host.fs != null
+    && ConstantsStateIsValid(host.constants)
+}
+
+
+predicate InitHostStatePostconditions(constants:ConstantsState, host:HostState)
+{
+       ConstantsStateIsAbstractable(constants)
+    && HostStateIsAbstractable(host)
+    && Host_Init(AbstractifyHostStateToHost(host), host.fs, AbstractifyEndPointToNodeIdentity(host.me), AbstractifyEndPointsToNodeIdentities(constants.hostIds), AbstractifyCParametersToParameters(constants.params))
+    && host.constants == constants
+    && HostStateIsValid(host)
+}
+
+predicate HostState_common_preconditions(host:HostState, cpacket:CPacket)
+{
+       HostStateIsAbstractable(host)
+    && CPacketIsAbstractable(cpacket)
+    && HostStateIsValid(host)
+}
+
+predicate HostState_common_postconditions(host:HostState, cpacket:CPacket, host':HostState, sent_packets:seq<CPacket>)
+{
+       HostState_common_preconditions(host, cpacket)
+    && HostStateIsAbstractable(host')
+    && host'.constants == host.constants
+    && host'.me == host.me
+    && CPacketSeqIsAbstractable(sent_packets)
+    && HostStateIsValid(host')
+    && OutboundPacketsSeqIsValid(sent_packets)
+    && OutboundPacketsSeqHasCorrectSrc(sent_packets, host.me)
+    && AbstractifySeqOfCPacketsToSetOfWsPackets(sent_packets) == ExtractPacketsFromLWSPackets(AbstractifyOutboundPacketsToSeqOfLWSPackets(sent_packets))
+}
+
+predicate NextGetRequestPreconditions(host:HostState, cpacket:CPacket)
+{
+       HostStateIsAbstractable(host)
+    && CPacketIsAbstractable(cpacket)
+    && cpacket.msg.CGetRequest?
+    && HostState_common_preconditions(host, cpacket)
+}
+predicate NextGetRequestPostconditions(host:HostState, cpacket:CPacket, host':HostState, sent_packets:seq<CPacket>)
+{
+       NextGetRequestPreconditions(host, cpacket)
+    && HostStateIsAbstractable(host')
+    && CPacketSeqIsAbstractable(sent_packets)
+    && NextGetRequest(AbstractifyHostStateToHost(host), AbstractifyHostStateToHost(host'), AbstractifyCPacketToWsPacket(cpacket), AbstractifySeqOfCPacketsToSetOfWsPackets(sent_packets))
+    && HostState_common_postconditions(host, cpacket, host', sent_packets)
+}
+}
